more conversions

Azurite/AzNat/Basic.lean
@@ -3,5 +3,8 @@ namespace Azurite
 structure AzNat where
   limbs : Array UInt64
   last_ne_zero : limbs.back? ≠ some 0
+  deriving DecidableEq
+
+instance : Inhabited AzNat := ⟨⟨#[], by simp⟩⟩
 
 end Azurite
