Azurite/AzNat/Conversion.lean
@@ -1,3 +1,4 @@
+import Azurite.AzNat.Parse
 import Azurite.AzNat.ToString
 
 def UInt64.toAzNat (u : UInt64) : Azurite.AzNat :=
@@ -43,3 +44,38 @@ def ISize.toAzNatClampNeg (i : ISize) : Azurite.AzNat := i.toInt64.toAzNatClampN
 
 #guard toString ((-5 : ISize).toAzNatClampNeg) == "0"
 #guard toString ((5 : ISize).toAzNatClampNeg) == "5"
+
+namespace Azurite.AzNat
+
+def toUInt64 (n : AzNat) : UInt64 :=
+  if h : n.limbs.size > 0 then n.limbs[0] else 0
+
+def toUInt32 (n : AzNat) : UInt32 := n.toUInt64.toUInt32
+def toUInt16 (n : AzNat) : UInt16 := n.toUInt64.toUInt16
+def toUInt8 (n : AzNat) : UInt8 := n.toUInt64.toUInt8
+def toUSize (n : AzNat) : USize := n.toUInt64.toUSize
+
+def toInt64 (n : AzNat) : Int64 := n.toUInt64.toInt64
+def toInt32 (n : AzNat) : Int32 := n.toUInt64.toUInt32.toInt32
+def toInt16 (n : AzNat) : Int16 := n.toUInt64.toUInt16.toInt16
+def toInt8 (n : AzNat) : Int8 := n.toUInt64.toUInt8.toInt8
+def toISize (n : AzNat) : ISize := n.toUInt64.toUSize.toISize
+
+end Azurite.AzNat
+
+#guard (Azurite.AzNat.parse "123".toList).get!.toUInt64 == 123
+#guard (Azurite.AzNat.parse "18446744073709551617".toList).get!.toUInt64 == 1
+#guard (Azurite.AzNat.parse "18446744073709551616".toList).get!.toInt64 == 0
+#guard (Azurite.AzNat.parse "9223372036854775808".toList).get!.toInt64 == -9223372036854775808
+
+#guard (Azurite.AzNat.parse "4294967297".toList).get!.toUInt32 == 1
+#guard (Azurite.AzNat.parse "4294967295".toList).get!.toInt32 == -1
+#guard (Azurite.AzNat.parse "2147483648".toList).get!.toInt32 == -2147483648
+
+#guard (Azurite.AzNat.parse "65537".toList).get!.toUInt16 == 1
+#guard (Azurite.AzNat.parse "65535".toList).get!.toInt16 == -1
+#guard (Azurite.AzNat.parse "32768".toList).get!.toInt16 == -32768
+
+#guard (Azurite.AzNat.parse "257".toList).get!.toUInt8 == 1
+#guard (Azurite.AzNat.parse "255".toList).get!.toInt8 == -1
+#guard (Azurite.AzNat.parse "128".toList).get!.toInt8 == -128
